work on flow to read a page from disk

examples/scache/RWLock.i.dfy
@@ -36,53 +36,76 @@ module RWLock refines ResourceBuilderSpec {
   type V = Handle
 
   /*
-   * We consider two bits of the status field, WriteLock and WriteBack.
-   * To avoid confusion, I simply call them 'Write' and 'Back'.
+   * We consider two bits of the status field, ExcLock and WriteBack.
    *
-   * Write and Back. Of course, 'Write'
-   * and 'Back' should be exclusive operations;
+   * ExcLock and WriteBack. Of course, 'ExcLock'
+   * and 'WriteBack' should be exclusive operations;
    * When both flags are set,
-   * it should be interpreted as the 'Write' being
-   * pending, with the 'Back' being in progress.
+   * it should be interpreted as the 'ExcLock' being
+   * pending, with the 'WriteBack' being active.
+   *
+   * Those 2 bits gives 2x2 = 4 states. We then have 2 more:
+   * Unmapped and Reading.
    */
   datatype Flag =
-    | Available
-    | Back
-    | Write
-    | Back_PendingWrite
     | Unmapped
+    | Reading
+    | Reading_ExcLock
+    | Available
+    | WriteBack
+    | ExcLock
+    | WriteBack_PendingExcLock
 
-  datatype WriteLockState = 
+  datatype ExcLockLockState = 
     | WLSNone
-    | WLSPendingAwaitBack
+    | WLSPendingAwaitWriteBack
     | WLSPending(visited: int)
     | WLSObtained
 
   datatype RWLockState = RWLockState(
-    writeLock: WriteLockState,
+    writeLock: ExcLockLockState,
     backHeld: bool,
     readCounts: seq<int>)
 
   datatype Q =
     | Global(g: map<Key, RWLockState>)
     | FlagsField(key: Key, flags: Flag)
-    | ReadRefCount(key: Key, t: int, refcount: uint8)
+    | SharedLockRefCount(key: Key, t: int, refcount: uint8)
 
-    | ReadPending(key: Key, t: int)
-    | ReadObtained(key: Key, t: int)
+    // Standard flow for obtained a 'shared' lock
+
+    | SharedLockPending(key: Key, t: int)
+    | SharedLockObtained(key: Key, t: int)
+
+    // Standard flow for obtained an 'exclusive' lock
+
+    | ExcLockPendingAwaitWriteBack(key: Key)
+    | ExcLockPending(key: Key, visited: int)
+    | ExcLockObtained(key: Key)
+
+    // Flow for the phase of reading in a page from disk.
+    // This is a special-case flow, because it needs to be performed
+    // on the way to obtaining a 'shared' lock, but it requires
+    // exclusive access to the underlying memory and resources.
+    // End-game for this flow is to become an ordinary 'shared' lock
+
+    | ReadingPending(key: Key)
+    | ReadingPendingCounted(key: Key, t: int)
+    | ReadingObtained(key: Key, t: int)
+
+    // Flow for the phase of doing a write-back.
+    // Special case in part because it can be initiated by any thread
+    // and completed by any thread (not necessarily the same one).
     
-    | BackObtained(key: Key)
+    | WriteBackObtained(key: Key)
 
-    | WritePendingAwaitBack(key: Key)
-    | WritePending(key: Key, visited: int)
-    | WriteObtained(key: Key)
 
   /*datatype QStep =
-    | TakeBackStep(key: Key)
-    | TakeWrite(key: Key)
-    | TakeWriteAwaitBack(key: Key)*/
+    | TakeWriteBackStep(key: Key)
+    | TakeExcLock(key: Key)
+    | TakeExcLockAwaitWriteBack(key: Key)*/
 
-  predicate TakeBack(a: multiset<R>, b: multiset<R>, key: Key,
+  predicate TakeWriteBack(a: multiset<R>, b: multiset<R>, key: Key,
       g: map<Key, RWLockState>, g': map<Key, RWLockState>)
   {
     && key in g
@@ -95,96 +118,96 @@ module RWLock refines ResourceBuilderSpec {
     }
     && b == multiset{
       Internal(Global(g')),
-      Internal(FlagsField(key, Back)),
-      Internal(BackObtained(key))
+      Internal(FlagsField(key, WriteBack)),
+      Internal(WriteBackObtained(key))
     }
   }
 
-  predicate TakeWrite(a: multiset<Q>, b: multiset<Q>, key: Key)
+  predicate TakeExcLock(a: multiset<Q>, b: multiset<Q>, key: Key)
   {
     && a == multiset{ FlagsField(key, Available) }
     && b == multiset{
-      FlagsField(key, Write),
-      WritePendingAwaitBack(key)
+      FlagsField(key, ExcLock),
+      ExcLockPendingAwaitWriteBack(key)
     }
   }
 
-  predicate TakeWriteAwaitBack(a: multiset<Q>, b: multiset<Q>, key: Key)
+  predicate TakeExcLockAwaitWriteBack(a: multiset<Q>, b: multiset<Q>, key: Key)
   {
-    && a == multiset{ FlagsField(key, Back) }
+    && a == multiset{ FlagsField(key, WriteBack) }
     && b == multiset{
-      FlagsField(key, Back_PendingWrite),
-      WritePendingAwaitBack(key)
+      FlagsField(key, WriteBack_PendingExcLock),
+      ExcLockPendingAwaitWriteBack(key)
     }
   }
 
-  predicate TakeWriteFinishBack(a: multiset<Q>, b: multiset<Q>, key: Key, fl: Flag)
+  predicate TakeExcLockFinishWriteBack(a: multiset<Q>, b: multiset<Q>, key: Key, fl: Flag)
   {
     // The 'free' case cannot actually occur, but it's convenient to allow it.
-    && (fl == Write || fl == Available)
+    && (fl == ExcLock || fl == Available)
     && a == multiset{
       FlagsField(key, fl),
-      WritePendingAwaitBack(key)
+      ExcLockPendingAwaitWriteBack(key)
     }
     && b == multiset{
       FlagsField(key, fl),
-      WritePending(key, 0)
+      ExcLockPending(key, 0)
     }
   }
 
-  predicate TakeWriteCheckReadZero(a: multiset<Q>, b: multiset<Q>, key: Key, idx: int)
+  predicate TakeExcLockCheckSharedLockZero(a: multiset<Q>, b: multiset<Q>, key: Key, idx: int)
   {
     && a == multiset{
-      WritePending(key, idx),
-      ReadRefCount(key, idx, 0) 
+      ExcLockPending(key, idx),
+      SharedLockRefCount(key, idx, 0) 
     }
     && b == multiset{
-      WritePending(key, idx + 1),
-      ReadRefCount(key, idx, 0) 
+      ExcLockPending(key, idx + 1),
+      SharedLockRefCount(key, idx, 0) 
     }
   }
 
-  predicate TakeWriteFinish(a: multiset<Q>, b: multiset<Q>, key: Key)
+  predicate TakeExcLockFinish(a: multiset<Q>, b: multiset<Q>, key: Key)
   {
     && a == multiset{
-      WritePending(key, NUM_THREADS)
+      ExcLockPending(key, NUM_THREADS)
     }
     && b == multiset{
-      WriteObtained(key)
+      ExcLockObtained(key)
     }
   }
 
-  predicate TakeRead(a: multiset<Q>, b: multiset<Q>, key: Key, t: int, r: uint8)
+  predicate TakeSharedLock(a: multiset<Q>, b: multiset<Q>, key: Key, t: int, r: uint8)
   {
     && a == multiset{
-      ReadRefCount(key, t, r)
+      SharedLockRefCount(key, t, r)
     }
     && a == multiset{
-      ReadRefCount(key, t, if r == 255 then 0 else r+1),
-      ReadPending(key, t)
+      SharedLockRefCount(key, t, if r == 255 then 0 else r+1),
+      SharedLockPending(key, t)
     }
   }
 
-  predicate TakeReadFinish(a: multiset<Q>, b: multiset<Q>, key: Key, t: int, r: uint8, fl: Flag)
+  predicate TakeSharedLockFinish(a: multiset<Q>, b: multiset<Q>, key: Key, t: int, r: uint8, fl: Flag)
   {
-    && (fl == Available || fl == Back)
+    && (fl == Available || fl == WriteBack)
     && a == multiset{
-      ReadPending(key, t),
+      SharedLockPending(key, t),
       FlagsField(key, fl)
     }
     && a == multiset{
-      ReadObtained(key, t)
+      SharedLockObtained(key, t)
     }
   }
 
-  predicate TakeReadBail(a: multiset<Q>, b: multiset<Q>, key: Key, t: int, r: uint8)
+  predicate TakeSharedLockBail(a: multiset<Q>, b: multiset<Q>, key: Key, t: int, r: uint8)
   {
     && a == multiset{
-      ReadRefCount(key, t, r),
-      ReadPending(key, t)
+      SharedLockRefCount(key, t, r),
+      SharedLockPending(key, t)
     }
     && b == multiset{
-      ReadRefCount(key, t, if r == 0 then 255 else r-1)
+      SharedLockRefCount(key, t, if r == 0 then 255 else r-1)
     }
   }
 
@@ -209,25 +232,25 @@ module RWLock refines ResourceBuilderSpec {
     && InvRWLockState(state)
     && (q.FlagsField? ==>
       && (q.flags == Available ==> state.writeLock == WLSNone && !state.backHeld)
-      && (q.flags == Back ==> state.writeLock == WLSNone && state.backHeld)
-      && (q.flags == Write ==> state.writeLock != WLSNone && !state.backHeld)
-      && (q.flags == Back_PendingWrite ==>
-          state.writeLock == WLSPendingAwaitBack && state.backHeld)
+      && (q.flags == WriteBack ==> state.writeLock == WLSNone && state.backHeld)
+      && (q.flags == ExcLock ==> state.writeLock != WLSNone && !state.backHeld)
+      && (q.flags == WriteBack_PendingExcLock ==>
+          state.writeLock == WLSPendingAwaitWriteBack && state.backHeld)
     )
-    && (q.ReadRefCount? ==>
+    && (q.SharedLockRefCount? ==>
       && 0 <= q.t < NUM_THREADS
       && state.readCounts[q.t] == q.refcount as int
     )
-    && (q.BackObtained? ==>
+    && (q.WriteBackObtained? ==>
       state.backHeld
     )
-    && (q.WritePendingAwaitBack? ==>
-      state.writeLock == WLSPendingAwaitBack
+    && (q.ExcLockPendingAwaitWriteBack? ==>
+      state.writeLock == WLSPendingAwaitWriteBack
     )
-    && (q.WritePending? ==>
+    && (q.ExcLockPending? ==>
       state.writeLock == WLSPending(q.visited)
     )
-    && (q.WriteObtained? ==>
+    && (q.ExcLockObtained? ==>
       state.writeLock == WLSObtained
     )
   }
@@ -246,11 +269,11 @@ module RWLock refines ResourceBuilderSpec {
     && r.Internal?
     && !(q.q.Global? && r.q.Global?)
     && (q.q.FlagsField? && r.q.FlagsField? ==> q.q.key != r.q.key)
-    && (q.q.ReadRefCount? && r.q.ReadRefCount? ==> !(q.q.key == r.q.key && q.q.t == r.q.t))
-    && (q.q.BackObtained? && r.q.BackObtained? ==> q.q.key != r.q.key)
-    && (q.q.WritePendingAwaitBack? && r.q.WritePendingAwaitBack? ==> q.q.key != r.q.key)
-    && (q.q.WritePending? && r.q.WritePending? ==> q.q.key != r.q.key)
-    && (q.q.WriteObtained? && r.q.WriteObtained? ==> q.q.key != r.q.key)
+    && (q.q.SharedLockRefCount? && r.q.SharedLockRefCount? ==> !(q.q.key == r.q.key && q.q.t == r.q.t))
+    && (q.q.WriteBackObtained? && r.q.WriteBackObtained? ==> q.q.key != r.q.key)
+    && (q.q.ExcLockPendingAwaitWriteBack? && r.q.ExcLockPendingAwaitWriteBack? ==> q.q.key != r.q.key)
+    && (q.q.ExcLockPending? && r.q.ExcLockPending? ==> q.q.key != r.q.key)
+    && (q.q.ExcLockObtained? && r.q.ExcLockObtained? ==> q.q.key != r.q.key)
     && (q.q.Global? ==>
       && InvObject(r, q.q.g)
     )
@@ -262,11 +285,11 @@ module RWLock refines ResourceBuilderSpec {
     && (forall a, b | multiset{a,b} <= s.m :: Inv2(a, b))
   }
 
-  lemma TakeBackPreservesInv(
+  lemma TakeWriteBackPreservesInv(
     s: Variables, s': Variables,
     a: multiset<R>, b: multiset<R>, c: multiset<R>,
     key: Key, g: map<Key, RWLockState>, g': map<Key, RWLockState>)
-  requires TakeBack(a, b, key, g, g')
+  requires TakeWriteBack(a, b, key, g, g')
   requires Inv(s)
   requires s.m == a + c
   requires s'.m == b + c
@@ -294,53 +317,82 @@ module RWLock refines ResourceBuilderSpec {
     assert Inv(s');
   }
 
-  method transform_TakeBack(key: Key, linear s: R)
+  method transform_TakeWriteBack(key: Key, linear s: R)
   returns (linear t: R, linear u: R, /*readonly*/ linear v: Handle)
   requires s == Internal(FlagsField(key, Available))
-  ensures t == Internal(FlagsField(key, Back))
-  ensures u == Internal(BackObtained(key))
+  ensures t == Internal(FlagsField(key, WriteBack))
+  ensures u == Internal(WriteBackObtained(key))
   ensures v.is_handle(key)
 
-  method transform_ReleaseBack(key: Key, fl: Flag,
+  method transform_ReleaseWriteBack(key: Key, fl: Flag,
     linear t: R, linear u: R, /*readonly*/ linear v: Handle)
   returns (linear s: R)
   requires t == Internal(FlagsField(key, fl))
-  requires u == Internal(BackObtained(key))
+  requires u == Internal(WriteBackObtained(key))
   requires v.is_handle(key)
-  ensures fl == Back || fl == Back_PendingWrite
-  ensures fl == Back ==> s == Internal(FlagsField(key, Available))
-  ensures fl == Back_PendingWrite ==> s == Internal(FlagsField(key, Write))
+  ensures fl == WriteBack || fl == WriteBack_PendingExcLock
+  ensures fl == WriteBack ==> s == Internal(FlagsField(key, Available))
+  ensures fl == WriteBack_PendingExcLock ==> s == Internal(FlagsField(key, ExcLock))
 
-  method transform_TakeWrite(key: Key, linear s: R)
+  method transform_TakeExcLock(key: Key, linear s: R)
   returns (linear t: R, linear u: R)
   requires s == Internal(FlagsField(key, Available))
-  ensures t == Internal(FlagsField(key, Write))
-  ensures u == Internal(WritePendingAwaitBack(key))
+  ensures t == Internal(FlagsField(key, ExcLock))
+  ensures u == Internal(ExcLockPendingAwaitWriteBack(key))
 
-  method transform_TakeWriteAwaitBack(key: Key, linear s: R)
+  method transform_TakeExcLockAwaitWriteBack(key: Key, linear s: R)
   returns (linear t: R, linear u: R)
-  requires s == Internal(FlagsField(key, Back))
-  ensures t == Internal(FlagsField(key, Back_PendingWrite))
-  ensures u == Internal(WritePendingAwaitBack(key))
+  requires s == Internal(FlagsField(key, WriteBack))
+  ensures t == Internal(FlagsField(key, WriteBack_PendingExcLock))
+  ensures u == Internal(ExcLockPendingAwaitWriteBack(key))
 
-  method transform_TakeWriteFinishBack(key: Key, fl: Flag, linear s1: R, linear s2: R)
+  method transform_TakeExcLockFinishWriteBack(key: Key, fl: Flag, linear s1: R, linear s2: R)
   returns (linear t1: R, linear t2: R)
-  requires fl == Write || fl == Available
+  requires fl == ExcLock || fl == Available
+      // vacuous cases:
+      || fl == Reading || fl == Reading_ExcLock || fl == Unmapped
   requires s1 == Internal(FlagsField(key, fl))
-  requires s2 == Internal(WritePendingAwaitBack(key))
+  requires s2 == Internal(ExcLockPendingAwaitWriteBack(key))
   ensures t1 == Internal(FlagsField(key, fl))
-  ensures t2 == Internal(WritePending(key, 0))
+  ensures t2 == Internal(ExcLockPending(key, 0))
 
-  method transform_TakeWriteCheckReadZero(key: Key, idx: int, linear s1: R, linear s2: R)
+  method transform_TakeExcLockCheckSharedLockZero(key: Key, idx: int, linear s1: R, linear s2: R)
   returns (linear t1: R, linear t2: R)
-  requires s1 == Internal(ReadRefCount(key, idx, 0))
-  requires s2 == Internal(WritePending(key, idx))
-  ensures t1 == Internal(ReadRefCount(key, idx, 0))
-  ensures t2 == Internal(WritePending(key, idx + 1))
+  requires s1 == Internal(SharedLockRefCount(key, idx, 0))
+  requires s2 == Internal(ExcLockPending(key, idx))
+  ensures t1 == Internal(SharedLockRefCount(key, idx, 0))
+  ensures t2 == Internal(ExcLockPending(key, idx + 1))
 
-  method transform_TakeWriteFinish(key: Key, linear s1: R)
+  method transform_TakeExcLockFinish(key: Key, linear s1: R)
   returns (linear t1: R, linear t2: Handle)
-  requires s1 == Internal(WritePending(key, NUM_THREADS))
-  ensures t1 == Internal(WriteObtained(key))
+  requires s1 == Internal(ExcLockPending(key, NUM_THREADS))
+  ensures t1 == Internal(ExcLockObtained(key))
   ensures t2.is_handle(key)
+
+  method transform_Alloc(key: Key, linear s1: R)
+  returns (linear t1: R, linear t2: R, linear handle: Handle)
+  requires s1 == Internal(FlagsField(key, Unmapped))
+  ensures t1 == Internal(FlagsField(key, Reading_ExcLock))
+  ensures t2 == Internal(ReadingPending(key))
+  ensures handle.is_handle(key)
+
+  method transform_ObtainReading(key: Key, t: int, fl: Flag,
+      linear s1: R, linear s2: R)
+  returns (linear t1: R, linear t2: R)
+  requires s1 == Internal(FlagsField(key, fl))
+  requires s2 == Internal(ReadingPendingCounted(key, t))
+  ensures t1 == Internal(FlagsField(key, Reading))
+  ensures t2 == Internal(ReadingObtained(key, t))
+
+  method transform_ReadingToShared(key: Key, t: int, fl: Flag,
+      linear s1: R, linear s2: R, linear handle: Handle)
+  returns (linear t1: R, linear t2: R, /*readonly*/ linear handle_out: Handle)
+  requires s1 == Internal(FlagsField(key, fl))
+  requires s2 == Internal(ReadingObtained(key, t))
+  requires handle.is_handle(key)
+  ensures fl == Reading
+  ensures t1 == Internal(FlagsField(key, Available))
+  ensures t2 == Internal(SharedLockObtained(key, t))
+  ensures handle_out == handle
+
 }
