examples/scache/AtomicStatus.i.dfy
@@ -11,17 +11,21 @@ module AtomicStatusImpl {
   import opened LinearMaybe
   import RWLock
 
-  const flag_empty : uint8 := 0;
+  const flag_zero : uint8 := 0;
 
-  const flag_back : uint8 := 1;
-  const flag_write : uint8 := 2;
+  const flag_writeback : uint8 := 1;
+  const flag_exc : uint8 := 2;
   const flag_accessed : uint8 := 4;
   const flag_unmapped : uint8 := 8;
+  const flag_reading : uint8 := 16;
 
-  const flag_back_write : uint8 := 3;
-  const flag_back_accessed : uint8 := 5;
+  const flag_writeback_exc : uint8 := 3;
+  const flag_writeback_accessed : uint8 := 5;
   const flag_write_accessed : uint8 := 6;
-  const flag_back_write_accessed : uint8 := 7;
+  const flag_writeback_exc_accessed : uint8 := 7;
+  const flag_accessed_reading : uint8 := 20;
+  const flag_exc_reading : uint8 := 18;
+  const flag_exc_accessed_reading : uint8 := 22;
 
   type AtomicStatus = Atomic<uint8, RWLock.R>
 
@@ -30,12 +34,14 @@ module AtomicStatusImpl {
     && g.Internal?
     && g.q.FlagsField?
     && g.q.key == key
-    && (g.q.flags == RWLock.Available ==> v == flag_empty || v == flag_accessed)
-    && (g.q.flags == RWLock.Back ==> v == flag_back || v == flag_back_accessed)
-    && (g.q.flags == RWLock.Write ==> v == flag_write || v == flag_write_accessed)
-    && (g.q.flags == RWLock.Back_PendingWrite ==>
-        v == flag_back_write || v == flag_back_write_accessed)
+    && (g.q.flags == RWLock.Available ==> v == flag_zero || v == flag_accessed)
+    && (g.q.flags == RWLock.WriteBack ==> v == flag_writeback || v == flag_writeback_accessed)
+    && (g.q.flags == RWLock.ExcLock ==> v == flag_exc || v == flag_write_accessed)
+    && (g.q.flags == RWLock.WriteBack_PendingExcLock ==>
+        v == flag_writeback_exc || v == flag_writeback_exc_accessed)
     && (g.q.flags == RWLock.Unmapped ==> v == flag_unmapped)
+    && (g.q.flags == RWLock.Reading ==> v == flag_reading || v == flag_accessed_reading)
+    && (g.q.flags == RWLock.Reading_ExcLock ==> v == flag_exc_reading || v == flag_exc_accessed_reading)
   }
 
   predicate atomic_status_inv(a: AtomicStatus, key: RWLock.Key)
@@ -53,23 +59,23 @@ module AtomicStatusImpl {
   requires atomic_status_inv(a, key)
   ensures !success ==> !has(m)
   ensures success ==> has(m)
-      && read(m) == RWLock.Internal(RWLock.BackObtained(key))
+      && read(m) == RWLock.Internal(RWLock.WriteBackObtained(key))
   ensures !success ==> !has(handle_out)
   ensures success ==> has(handle_out)
       && read(handle_out).is_handle(key)
   {
     var cur_flag := atomic_read(a);
-    if !(cur_flag == flag_empty || (with_access && cur_flag == flag_accessed)) {
+    if !(cur_flag == flag_zero || (with_access && cur_flag == flag_accessed)) {
       m := empty();
       handle_out := empty();
       success := false;
     } else {
-      var did_set := compare_and_set(a, flag_empty, flag_back);
+      var did_set := compare_and_set(a, flag_zero, flag_writeback);
 
       ///// Begin jank
       ///// Setup:
-      var v1 := flag_empty;
-      var v2 := flag_back;
+      var v1 := flag_zero;
+      var v2 := flag_writeback;
       var old_v: uint8;
       var new_v: uint8;
       linear var old_g: RWLock.R := unsafe_obtain();
@@ -80,7 +86,7 @@ module AtomicStatusImpl {
       ///// Transfer:
       if did_set {
         linear var res, handle;
-        new_g, res, handle := RWLock.transform_TakeBack(key, old_g);
+        new_g, res, handle := RWLock.transform_TakeWriteBack(key, old_g);
         handle_out := give(handle);
         m := give(res);
       } else {
@@ -99,12 +105,12 @@ module AtomicStatusImpl {
       } else if !with_access {
         success := false;
       } else {
-        var did_set := compare_and_set(a, flag_accessed, flag_back_accessed);
+        var did_set := compare_and_set(a, flag_accessed, flag_writeback_accessed);
 
         ///// Begin jank
         ///// Setup:
         var v1 := flag_accessed;
-        var v2 := flag_back_accessed;
+        var v2 := flag_writeback_accessed;
         var old_v: uint8;
         var new_v: uint8;
         linear var old_g: RWLock.R := unsafe_obtain();
@@ -118,7 +124,7 @@ module AtomicStatusImpl {
 
         if did_set {
           linear var res, handle;
-          new_g, res, handle := RWLock.transform_TakeBack(key, old_g);
+          new_g, res, handle := RWLock.transform_TakeWriteBack(key, old_g);
           handle_out := give(handle);
           m := give(res);
         } else {
@@ -141,14 +147,14 @@ module AtomicStatusImpl {
       linear r: RWLock.R,
       /* readonly */ linear handle: RWLock.Handle)
   requires atomic_status_inv(a, key)
-  requires r == RWLock.Internal(RWLock.BackObtained(key))
+  requires r == RWLock.Internal(RWLock.WriteBackObtained(key))
   requires handle.is_handle(key)
   {
-    var orig_value := fetch_and(a, 0xff - flag_back);
+    var orig_value := fetch_and(a, 0xff - flag_writeback);
 
     ///// Begin jank
     ///// Setup:
-    var v := 0xff - flag_back;
+    var v := 0xff - flag_writeback;
     var old_v: uint8;
     var new_v: uint8;
     linear var old_g: RWLock.R := unsafe_obtain();
@@ -158,7 +164,7 @@ module AtomicStatusImpl {
     linear var new_g;
     ///// Transfer:
     var fl := old_g.q.flags;
-    new_g := RWLock.transform_ReleaseBack(key, fl, old_g, r, handle);
+    new_g := RWLock.transform_ReleaseWriteBack(key, fl, old_g, r, handle);
 
     assert state_inv(new_v, new_g, key);
     ///// Teardown:
@@ -167,18 +173,18 @@ module AtomicStatusImpl {
     ///// End jank
   }
 
-  method try_set_write_lock(a: AtomicStatus, key: RWLock.Key)
+  /*method try_set_write_lock(a: AtomicStatus, key: RWLock.Key)
   returns (success: bool, linear m: maybe<RWLock.R>)
   requires atomic_status_inv(a, key)
   ensures !success ==> !has(m)
   ensures success ==> has(m)
-      && read(m) == RWLock.Internal(RWLock.WritePendingAwaitBack(key))
+      && read(m) == RWLock.Internal(RWLock.ExcLockPendingAwaitWriteBack(key))
   {
-    var orig_value := fetch_or(a, flag_write);
+    var orig_value := fetch_or(a, flag_exc);
 
     ///// Begin jank
     ///// Setup:
-    var v := flag_write;
+    var v := flag_exc;
     var old_v: uint8;
     var new_v: uint8;
     linear var old_g: RWLock.R := unsafe_obtain();
@@ -190,11 +196,11 @@ module AtomicStatusImpl {
     var fl := old_g.q.flags;
     if fl == RWLock.Available {
       linear var r;
-      new_g, r := RWLock.transform_TakeWrite(key, old_g);
+      new_g, r := RWLock.transform_TakeExcLock(key, old_g);
       m := give(r);
-    } else if fl == RWLock.Back {
+    } else if fl == RWLock.WriteBack {
       linear var r;
-      new_g, r := RWLock.transform_TakeWriteAwaitBack(key, old_g);
+      new_g, r := RWLock.transform_TakeExcLockAwaitWriteBack(key, old_g);
       m := give(r);
     } else {
       new_g := old_g;
@@ -205,16 +211,16 @@ module AtomicStatusImpl {
     unsafe_dispose(new_g);
     ///// End jank
 
-    success := bit_and(orig_value, flag_write) == 0;
-  }
+    success := bit_and(orig_value, flag_exc) == 0;
+  }*/
 
   method try_check_writeback_isnt_set(a: AtomicStatus, key: RWLock.Key,
       linear m: RWLock.R)
   returns (success: bool, linear m': RWLock.R)
   requires atomic_status_inv(a, key)
-  requires m == RWLock.Internal(RWLock.WritePendingAwaitBack(key))
+  requires m == RWLock.Internal(RWLock.ExcLockPendingAwaitWriteBack(key))
   ensures !success ==> m' == m
-  ensures success ==> m' == RWLock.Internal(RWLock.WritePending(key, 0))
+  ensures success ==> m' == RWLock.Internal(RWLock.ExcLockPending(key, 0))
   {
     var f := atomic_read(a);
 
@@ -230,9 +236,12 @@ module AtomicStatusImpl {
     ///// Transfer:
     var fl := old_g.q.flags;
     if fl == RWLock.Available
-        || fl == RWLock.Write
+        || fl == RWLock.ExcLock
+        || fl == RWLock.Reading
+        || fl == RWLock.Reading_ExcLock
+        || fl == RWLock.Unmapped
     {
-      new_g, m' := RWLock.transform_TakeWriteFinishBack(key, fl, old_g, m);
+      new_g, m' := RWLock.transform_TakeExcLockFinishWriteBack(key, fl, old_g, m);
     } else {
       new_g := old_g;
       m' := m;
@@ -242,6 +251,119 @@ module AtomicStatusImpl {
     unsafe_dispose(new_g);
     ///// End jank
 
-    success := bit_and(f, flag_back) == 0;
+    success := bit_and(f, flag_writeback) == 0;
+  }
+
+  method try_alloc(a: AtomicStatus, key: RWLock.Key)
+  returns (success: bool,
+      linear m: maybe<RWLock.R>,
+      linear handle_maybe: maybe<RWLock.Handle>)
+  requires atomic_status_inv(a, key)
+  ensures !success ==> !has(m)
+  ensures success ==> has(m)
+      && read(m) == RWLock.Internal(RWLock.ReadingPending(key))
+  ensures !success ==> !has(handle_maybe)
+  ensures success ==> has(handle_maybe)
+      && read(handle_maybe).is_handle(key)
+  {
+    // check first to reduce contention
+    var f := atomic_read(a);
+    if f != flag_unmapped {
+      success := false;
+      m := empty();
+      handle_maybe := empty();
+    } else {
+      var did_set := compare_and_set(a, flag_unmapped, flag_exc_reading);
+
+      ///// Begin jank
+      ///// Setup:
+      var v1 := flag_unmapped;
+      var v2 := flag_exc_reading;
+      var old_v: uint8;
+      var new_v: uint8;
+      linear var old_g: RWLock.R := unsafe_obtain();
+      assume old_v == v1 ==> new_v == v2 && did_set;
+      assume old_v != v1 ==> new_v == old_v && !did_set;
+      assume atomic_inv(a, old_v, old_g);
+      linear var new_g;
+      ///// Transfer:
+      if did_set {
+        linear var res, handle;
+        new_g, res, handle := RWLock.transform_Alloc(key, old_g);
+        m := give(res);
+        handle_maybe := give(handle);
+      } else {
+        m := empty();
+        handle_maybe := empty();
+        new_g := old_g;
+      }
+      assert state_inv(new_v, new_g, key);
+      ///// Teardown:
+      assert atomic_inv(a, new_v, new_g);
+      unsafe_dispose(new_g);
+      ///// End jank
+
+      success := did_set;
+    }
+  }
+
+  method clear_exc_bit_during_load_phase(a: AtomicStatus, key: RWLock.Key, t:int,
+      linear r: RWLock.R)
+  returns (linear q: RWLock.R)
+  requires atomic_status_inv(a, key)
+  requires r == RWLock.Internal(RWLock.ReadingPendingCounted(key, t))
+  ensures q == RWLock.Internal(RWLock.ReadingObtained(key, t))
+  {
+    atomic_write(a, flag_accessed_reading); // TODO 'clean' bit
+
+    ///// Begin jank
+    ///// Setup:
+    var v := flag_accessed_reading;
+    var old_v: uint8;
+    var new_v: uint8;
+    linear var old_g: RWLock.R := unsafe_obtain();
+    assume new_v == v;
+    assume atomic_inv(a, old_v, old_g);
+    linear var new_g;
+    ///// Transfer:
+    var fl := old_g.q.flags;
+    new_g, q := RWLock.transform_ObtainReading(key, t, fl, old_g, r);
+    ///// Teardown:
+    assert atomic_inv(a, new_v, new_g);
+    unsafe_dispose(new_g);
+    ///// End jank
+  }
+
+  method load_phase_finish(a: AtomicStatus, key: RWLock.Key, t: int,
+      linear r: RWLock.R, linear handle: RWLock.Handle)
+  returns (linear q: RWLock.R, /*readonly*/ linear handle_out: RWLock.Handle)
+  requires atomic_status_inv(a, key)
+  requires r == RWLock.Internal(RWLock.ReadingObtained(key, t))
+  requires handle.is_handle(key)
+  ensures q == RWLock.Internal(RWLock.SharedLockObtained(key, t))
+  ensures handle_out == handle
+  {
+    var orig_value := fetch_and(a, 0xff - flag_reading);
+
+    ///// Begin jank
+    ///// Setup:
+    var v := 0xff - flag_reading;
+    var old_v: uint8;
+    var new_v: uint8;
+    linear var old_g: RWLock.R := unsafe_obtain();
+    assume orig_value == old_v;
+    assume new_v == bit_and(old_v, v);
+    assume atomic_inv(a, old_v, old_g);
+    linear var new_g;
+    ///// Transfer:
+    var fl := old_g.q.flags;
+    new_g, q, handle_out :=
+        RWLock.transform_ReadingToShared(key, t, fl, old_g, r, handle);
+
+    assert state_inv(new_v, new_g, key);
+    ///// Teardown:
+    assert atomic_inv(a, new_v, new_g);
+    unsafe_dispose(new_g);
+    ///// End jank
   }
 }
